work: proof of 2-sat main theorem

SeparationLogic/algorithms/TwoSAT/TwoSAT.v
@@ -7,13 +7,73 @@ Require Import Coq.Logic.IndefiniteDescription.
 Require Import Coq.Logic.FunctionalExtensionality.
 Require Import Coq.micromega.Lia.
 Require Import Recdef.
+Require Import SetsClass.
 Require Import GraphLib.graph_basic.
+Require Import GraphLib.reachable.reachable_basic.
 Require Import GraphLib.Syntax.
-Require Import GraphLib.examples.tarjan.
-Require Import Algorithms.Tarjan_directed.SCC_basic.
+Require Import Algorithms.Kosaraju.SCC.
 Import ListNotations.
 
 Local Open Scope Z_scope.
+
+(* ================================================================ *)
+(* DiGraph: Record for directed graphs, used by Kosaraju.SCC       *)
+(* ================================================================ *)
+
+Record DiGraph (V E : Type) : Type := {
+  dig_vvalid : V -> Prop;
+  dig_evalid : E -> Prop;
+  dig_fst : E -> V;
+  dig_snd : E -> V;
+  dig_listV : list V;
+}.
+
+Arguments dig_vvalid {V E} _ _.
+Arguments dig_evalid {V E} _ _.
+Arguments dig_fst {V E} _ _.
+Arguments dig_snd {V E} _ _.
+Arguments dig_listV {V E} _.
+
+Record dig_step_aux {V E} (g : DiGraph V E) (e : E) (x y : V) : Prop := DigStepAux {
+  dsa_valid_edge : dig_evalid g e;
+  dsa_valid_src  : dig_vvalid g x;
+  dsa_valid_tgt  : dig_vvalid g y;
+  dsa_fst_eq     : dig_fst g e = x;
+  dsa_snd_eq     : dig_snd g e = y;
+}.
+
+Arguments dig_step_aux {V E} _ _ _ _.
+
+#[export] Instance dig_Graph (V E : Type) : Graph (DiGraph V E) V E := {|
+  vvalid   := fun g v   => dig_vvalid g v;
+  evalid   := fun g e   => dig_evalid g e;
+  step_aux := fun g e x y => dig_step_aux g e x y;
+|}.
+
+Record DiGraphProp (V E : Type) (g : DiGraph V E) : Prop := {
+  dgp_fst_valid     : forall e, dig_evalid g e -> dig_vvalid g (dig_fst g e);
+  dgp_snd_valid     : forall e, dig_evalid g e -> dig_vvalid g (dig_snd g e);
+  dgp_list_complete : forall v, dig_vvalid g v -> In v (dig_listV g);
+}.
+
+#[export] Instance dig_GValid (V E : Type) : GValid (DiGraph V E) :=
+  @DiGraphProp V E.
+
+#[export] Instance dig_StepValid (V E : Type) : StepValid (DiGraph V E) V E.
+Proof.
+  split; intros g e x y Hstep.
+  - destruct Hstep as [He Hx Hy Hfx Hsy]; exact Hx.
+  - destruct Hstep as [He Hx Hy Hfx Hsy]; exact Hy.
+  - destruct Hstep as [He Hx Hy Hfx Hsy]; exact He.
+Defined.
+
+#[export] Instance dig_FiniteGraph (V E : Type) : FiniteGraph (DiGraph V E) V E.
+Proof.
+  refine {| listV := dig_listV; |}.
+  intros g Hg Hv.
+  destruct (Hg : DiGraphProp V E g) as [_ _ Hcomplete].
+  apply Hcomplete; auto.
+Defined.
 
 (* ================================================================ *)
 (* Section 1: 2-SAT Syntax                                          *)
@@ -117,20 +177,19 @@ Qed.
 Definition nth_clause (f : formula) (i : Z) : clause :=
   nth (Z.to_nat i) f ((0, false), (0, false)).
 
-Definition implication_graph (f : formula) (numVars : Z)
-  : OriginalGraphType literal Z :=
+Definition implication_graph (f : formula) (numVars : Z) : DiGraph literal Z :=
   {|
-    original_vvalid := fun (l : literal) => valid_literal numVars l;
-    original_step := fun (e : Z) => 0 <= e < 2 * Zlength f;
-    original_step_fst := fun (e : Z) =>
+    dig_vvalid := fun (l : literal) => valid_literal numVars l;
+    dig_evalid := fun (e : Z) => 0 <= e < 2 * Zlength f;
+    dig_fst := fun (e : Z) =>
       let i := e / 2 in
       let c := nth_clause f i in
       if Z.even e then negate (fst c) else negate (snd c);
-    original_step_snd := fun (e : Z) =>
+    dig_snd := fun (e : Z) =>
       let i := e / 2 in
       let c := nth_clause f i in
       if Z.even e then snd c else fst c;
-    original_listV := literal_list numVars;
+    dig_listV := literal_list numVars;
   |}.
 
 Lemma nth_clause_in : forall f i, 0 <= i < Zlength f ->
@@ -145,105 +204,138 @@ Qed.
 
 Lemma implication_graph_gvalid : forall f numVars,
   valid_formula numVars f ->
-  OriginalGraphProp literal Z (implication_graph f numVars).
+  DiGraphProp literal Z (implication_graph f numVars).
 Proof.
   intros f numVars Hvalid.
   set (g := implication_graph f numVars).
-  constructor; unfold g; simpl; intros.
-  - unfold valid_literal.
-    destruct (Z.even e) eqn: Heven;
-      [ apply valid_literal_negate | apply valid_literal_negate ];
-      unfold Z.mul in H; destruct H as [He1 He2];
-      assert (Hdiv : 0 <= e / 2 < Zlength f)
-        by (split; [apply Z.div_pos; [exact He1 | lia] |
-                    apply Z.div_lt_upper_bound; [lia | exact He2]]);
-      destruct (Hvalid _ (nth_clause_in f (e / 2) Hdiv)) as [Hl1 Hl2];
-      auto.
-  - unfold valid_literal.
-    destruct (Z.even e) eqn: Heven;
-      unfold Z.mul in H; destruct H as [He1 He2].
-    + assert (Hdiv : 0 <= e / 2 < Zlength f)
-        by (split; [apply Z.div_pos; [exact He1 | lia] |
-                    apply Z.div_lt_upper_bound; [lia | exact He2]]);
-      destruct (Hvalid _ (nth_clause_in f (e / 2) Hdiv)) as [_ Hl2]; auto.
-    + assert (Hdiv : 0 <= e / 2 < Zlength f)
-        by (split; [apply Z.div_pos; [exact He1 | lia] |
-                    apply Z.div_lt_upper_bound; [lia | exact He2]]);
-      destruct (Hvalid _ (nth_clause_in f (e / 2) Hdiv)) as [Hl1 _]; auto.
-  - apply literal_list_complete; auto.
+  constructor.
+  - intros e He.
+    unfold g, implication_graph; simpl in *.
+    destruct He as [He1 He2].
+    set (i := e / 2).
+    assert (Hi_range : 0 <= i < Zlength f)
+      by (split; [apply Z.div_pos; [exact He1 | lia] |
+                  apply Z.div_lt_upper_bound; [lia | exact He2]]).
+    destruct (Z.even e) eqn: Heven; simpl.
+    + apply valid_literal_negate.
+      destruct (Hvalid (nth_clause f i) (nth_clause_in f i Hi_range)) as [Hl1 _].
+      exact Hl1.
+    + apply valid_literal_negate.
+      destruct (Hvalid (nth_clause f i) (nth_clause_in f i Hi_range)) as [_ Hl2].
+      exact Hl2.
+  - intros e He.
+    unfold g, implication_graph; simpl in *.
+    destruct He as [He1 He2].
+    set (i := e / 2).
+    assert (Hi_range : 0 <= i < Zlength f)
+      by (split; [apply Z.div_pos; [exact He1 | lia] |
+                  apply Z.div_lt_upper_bound; [lia | exact He2]]).
+    destruct (Z.even e) eqn: Heven; simpl.
+    + destruct (Hvalid (nth_clause f i) (nth_clause_in f i Hi_range)) as [_ Hl2].
+      exact Hl2.
+    + destruct (Hvalid (nth_clause f i) (nth_clause_in f i Hi_range)) as [Hl1 _].
+      exact Hl1.
+  - intros v Hv.
+    unfold g, implication_graph; simpl in *.
+    apply literal_list_complete; auto.
 Qed.
 
-Lemma dg_step_implication : forall f numVars c,
-  In c f ->
-  dg_step (implication_graph f numVars) (negate (fst c)) (snd c) /\
-  dg_step (implication_graph f numVars) (negate (snd c)) (fst c).
+Lemma step_implication : forall f numVars,
+  valid_formula numVars f ->
+  forall c, In c f ->
+  step (implication_graph f numVars) (negate (fst c)) (snd c) /\
+  step (implication_graph f numVars) (negate (snd c)) (fst c).
 Proof.
-  intros f numVars [l1 l2] Hc.
+  intros f numVars Hvalid [l1 l2] Hc.
   set (g := implication_graph f numVars).
   assert (Hpos: exists i : Z, 0 <= i < Zlength f /\
     nth (Z.to_nat i) f ((0,false),(0,false)) = (l1, l2)).
   { apply In_nth with (d := ((0,false),(0,false))) in Hc.
     destruct Hc as [i [Hrange Hnth]].
     exists (Z.of_nat i); split.
-    - split.
-      + apply (Nat2Z.is_nonneg i).
-      + apply Nat2Z.inj_lt in Hrange.
-        rewrite Zlength_correct.
-        assumption.
+    - split; [apply (Nat2Z.is_nonneg i) |].
+      apply Nat2Z.inj_lt in Hrange.
+      rewrite Zlength_correct; assumption.
     - rewrite Nat2Z.id; auto. }
   destruct Hpos as [i [Hrange Hnth]].
-  unfold g, implication_graph; simpl.
   pose (e1 := 2 * i).
   pose (e2 := 2 * i + 1).
-  assert (Hstep1: original_step g e1).
-  { unfold original_step, e1.
-    rewrite Zlength_correct in Hrange.
+  assert (He1_valid : dig_evalid g e1).
+  { unfold g, implication_graph.
+    unfold e1; destruct Hrange as [Hlow Hhigh].
+    split; [lia | apply Zmult_lt_compat_l; [lia | exact Hhigh]]. }
+  assert (He2_valid : dig_evalid g e2).
+  { unfold g, implication_graph.
+    unfold e2; destruct Hrange as [Hlow Hhigh].
     split; [lia |].
-    rewrite Zlength_correct; lia. }
-  assert (Hstep2: original_step g e2).
-  { unfold original_step, e2.
-    rewrite Zlength_correct in Hrange.
-    split; [lia |].
-    rewrite Zlength_correct; lia. }
-  split.
-  - unfold dg_step.
-    exists e1; split; [exact Hstep1 |].
-    unfold original_step_fst, original_step_snd, e1, nth_clause.
-    assert (Hdiv : (2*i)/2 = i).
-    { symmetry; apply Z.div_unique with (r := 0); [lia | ring]. }
-    rewrite Hdiv.
-    assert (Heven : Z.even (2*i) = true) by (rewrite Z.even_mul, Z.even_2; auto).
-    rewrite Heven; rewrite Hnth; auto.
-  - unfold dg_step.
-    exists e2; split; [exact Hstep2 |].
-    unfold original_step_fst, original_step_snd, e2, nth_clause.
-    assert (Hdiv : (2*i+1)/2 = i).
-    { rewrite Z.mul_comm.
-      rewrite Z.div_add_l by lia.
-      rewrite Z.div_small; [ring | lia]. }
-    rewrite Hdiv.
-    assert (Heven : Z.even (2*i+1) = false) by
-      (rewrite Z.even_add, Z.even_mul, Z.even_2; simpl; auto).
-    rewrite Heven; rewrite Hnth; auto.
+    apply Z.lt_le_trans with (2 * (i + 1)).
+    - nia.
+    - apply Zmult_le_compat_l; [lia |].
+      nia. }
+  assert (Hvalid_c : valid_clause numVars (l1, l2)) by (apply Hvalid; exact Hc).
+  destruct Hvalid_c as [Hvalid_l1 Hvalid_l2].
+  assert (Hstep1 : step g (negate l1) l2).
+  { unfold step; exists e1.
+    apply (DigStepAux literal Z g e1 (negate l1) l2 He1_valid
+      (valid_literal_negate numVars l1 Hvalid_l1) Hvalid_l2).
+    - unfold g, implication_graph, dig_fst; simpl.
+      unfold e1, nth_clause.
+      rewrite (Z.mul_comm 2 i), Z.div_mul by lia.
+      rewrite Z.even_mul, Z.even_2; simpl.
+      rewrite Bool.orb_true_r; simpl.
+      rewrite Hnth; reflexivity.
+    - unfold g, implication_graph, dig_snd; simpl.
+      unfold e1, nth_clause.
+      rewrite (Z.mul_comm 2 i), Z.div_mul by lia.
+      rewrite Z.even_mul, Z.even_2; simpl.
+      rewrite Bool.orb_true_r; simpl.
+      rewrite Hnth; reflexivity. }
+  assert (Hstep2 : step g (negate l2) l1).
+  { unfold step; exists e2.
+    assert (e2_div_2_eq_i : e2 / 2 = i).
+    { unfold e2. rewrite (Z.mul_comm 2 i), Z.div_add_l by lia.
+      rewrite Z.div_small; [|lia]. ring. }
+    assert (e2_even_false : Z.even e2 = false).
+    { unfold e2. apply Z.even_odd. }
+    apply (DigStepAux literal Z g e2 (negate l2) l1 He2_valid
+      (valid_literal_negate numVars l2 Hvalid_l2) Hvalid_l1).
+    - unfold g, implication_graph, dig_fst; simpl.
+      unfold nth_clause.
+      rewrite e2_div_2_eq_i.
+      rewrite e2_even_false; simpl.
+      rewrite Hnth; reflexivity.
+    - unfold g, implication_graph, dig_snd; simpl.
+      unfold nth_clause.
+      rewrite e2_div_2_eq_i.
+      rewrite e2_even_false; simpl.
+      rewrite Hnth; reflexivity.
+  }
+  split; [exact Hstep1 | exact Hstep2].
 Qed.
 
 (* ================================================================ *)
 (* Section 4: Forward Direction                                      *)
 (* ================================================================ *)
 
+Definition mutually_reachable (g : DiGraph literal Z) (u v : literal) : Prop :=
+  reachable g u v /\ reachable g v u.
+
+Definition no_conflict (g : DiGraph literal Z) (numVars : Z) : Prop :=
+  forall v, 1 <= v <= numVars ->
+    ~ mutually_reachable g (v, true) (v, false).
+
 Lemma eval_preserved_along_step : forall f numVars a,
   satisfies a f ->
   forall l1 l2,
-  dg_step (implication_graph f numVars) l1 l2 ->
+  step (implication_graph f numVars) l1 l2 ->
   eval_literal a l1 = true -> eval_literal a l2 = true.
 Proof.
   intros f numVars a Hsat l1 l2 Hstep Heval.
   set (g := implication_graph f numVars) in *.
-  destruct Hstep as [e [Hstep [Hfst Hsnd]]].
-  unfold g in Hfst, Hsnd, Hstep.
-  cbv zeta in Hfst, Hsnd, Hstep.
-  simpl in Hfst, Hsnd.
-  rename Hstep into Hrange.
+  destruct Hstep as [e Hstep].
+  destruct Hstep as [He Hx Hy Hfx Hsy].
+  unfold g, implication_graph in Hfx, Hsy; simpl in Hfx, Hsy.
+  rename He into Hrange.
   destruct Hrange as [He1 He2].
   set (i := e / 2).
   set (c := nth_clause f i).
@@ -251,21 +343,16 @@ Proof.
   { unfold i; split.
     - apply Z.div_pos; [exact He1 | apply Z.lt_0_2].
     - apply Z.div_lt_upper_bound; [apply Z.lt_0_2 | exact He2]. }
-  revert Hfst Hsnd.
-  destruct (Z.even e) eqn: Heven;
-    intros Hfst Hsnd;
-    simpl in Hfst, Hsnd.
-  - (* Z.even e = true *)
-    unfold c, i in Hfst, Hsnd.
-    rewrite <- Hfst in Heval; rewrite <- Hsnd.
+  revert Hfx Hsy.
+  destruct (Z.even e) eqn: Heven; intros Hfx Hsy; simpl in Hfx, Hsy;
+    unfold c, i in Hfx, Hsy.
+  - rewrite <- Hfx in Heval; rewrite <- Hsy.
     rewrite eval_negate in Heval.
     destruct (Hsat (nth_clause f (e/2)) (nth_clause_in f i Hi_range))
       as [Hc1 | Hc2].
     + rewrite Hc1 in Heval; simpl in Heval; discriminate.
     + exact Hc2.
-  - (* Z.even e = false *)
-    unfold c, i in Hfst, Hsnd.
-    rewrite <- Hfst in Heval; rewrite <- Hsnd.
+  - rewrite <- Hfx in Heval; rewrite <- Hsy.
     rewrite eval_negate in Heval.
     destruct (Hsat (nth_clause f (e/2)) (nth_clause_in f i Hi_range))
       as [Hc1 | Hc2].
@@ -276,19 +363,26 @@ Qed.
 Lemma eval_preserved_along_path : forall f numVars a,
   satisfies a f ->
   forall l1 l2,
-  dg_reachable (implication_graph f numVars) l1 l2 ->
+  reachable (implication_graph f numVars) l1 l2 ->
   eval_literal a l1 = true -> eval_literal a l2 = true.
 Proof.
   intros f numVars a Hsat l1 l2 Hreach Heval.
-  induction Hreach.
-  - apply (eval_preserved_along_step f numVars a Hsat x y H Heval).
-  - exact Heval.
-  - apply IHHreach2; apply IHHreach1; exact Heval.
+  unfold reachable in Hreach.
+  unfold reachable in Hreach.
+  let X := eval unfold clos_refl_trans in Hreach in
+  change Hreach with X.
+  destruct Hreach as [n Hn].
+  induction n as [| n IH] in l1, l2, Hn, Heval |- *.
+  - simpl nsteps in Hn.
+    unfold Rels.id in Hn.
+    simpl in Hn.
+    subst; exact Heval.
+  - simpl nsteps in Hn.
+    unfold Rels.concat in Hn.
+    destruct Hn as [z [Hz1 Hz2]].
+    apply (IH z l2 Hz2).
+    apply (eval_preserved_along_step f numVars a Hsat l1 z Hz1 Heval).
 Qed.
-
-Definition no_conflict (g : OriginalGraphType literal Z) (numVars : Z) : Prop :=
-  forall v, 1 <= v <= numVars ->
-    ~ mutually_reachable g (v, true) (v, false).
 
 Lemma forward : forall f numVars,
   valid_formula numVars f ->
@@ -328,15 +422,129 @@ Section BACKWARD.
 Variables (f : formula) (numVars : Z).
 Hypothesis (Hvalid : valid_formula numVars f).
 
-Let g : OriginalGraphType literal Z := implication_graph f numVars.
-Let Hgvalid : OriginalGraphProp literal Z g :=
-  implication_graph_gvalid f numVars Hvalid.
-Let Hfinite : forall v : literal, original_vvalid g v -> In v (original_listV g) :=
-  literal_list_complete numVars.
+Let g : DiGraph literal Z := implication_graph f numVars.
 
-Let Hsccp : exists sccs, scc_partition g sccs :=
-  scc_partition_exists g Hgvalid Hfinite.
+Let Hgvalid_g : gvalid g := implication_graph_gvalid f numVars Hvalid.
 
+Lemma backward (Hnc : no_conflict g numVars) : satisfiable f.
+Proof.
+  destruct (scc_partition_exists g (Hgvalid := Hgvalid_g))
+    as [sccs [[Hcover [Hisscc Hdisjoint]] Hnodup]].
+  destruct (exists_topological_order g sccs
+              (conj Hcover (conj Hisscc Hdisjoint)) Hnodup)
+    as [prec [Hcond_edge [Htotal [Hirrefl Htrans]]]].
+  set (scc_of := fun (l : literal) =>
+    epsilon (inhabits (fun (_ : literal) => True)) (fun s : literal -> Prop => In s sccs /\ s l)).
+  assert (scc_of_spec : forall (l : literal), valid_literal numVars l ->
+    In (scc_of l) sccs /\ (scc_of l) l).
+  { intros l Hv; unfold scc_of.
+    assert (Hex : exists s, In s sccs /\ s l) by (apply Hcover; auto).
+    exact (epsilon_spec (inhabits (fun (_ : literal) => True))
+      (fun s : literal -> Prop => In s sccs /\ s l) Hex). }
+  assert (scc_of_neq : forall (v : Z), 1 <= v <= numVars ->
+    scc_of (v, true) <> scc_of (v, false)).
+  { intros v Hv_range Heq.
+    apply (Hnc v Hv_range).
+    assert (Hscc : is_SCC g (scc_of (v, true))) by
+      (apply Hisscc; eapply scc_of_spec; eauto; exact (conj Hv_range eq_refl)).
+    destruct Hscc as [_ [Hmr _]].
+    apply (Hmr (v, true) (v, false));
+      [eapply scc_of_spec; eauto; exact (conj Hv_range eq_refl)
+      | rewrite Heq; eapply scc_of_spec; eauto; exact (conj Hv_range eq_refl)]. }
+  set (a := fun (v : Z) =>
+    if excluded_middle_informative (1 <= v <= numVars) then
+      if excluded_middle_informative (prec (scc_of (v, false)) (scc_of (v, true)))
+      then true else false
+    else false).
+  assert (eval_false_prec : forall (l : literal) (Hv : valid_literal numVars l),
+    eval_literal a l = false -> prec (scc_of l) (scc_of (negate l))).
+  { intros l Hv Hfalse.
+    destruct l as [v b]; destruct b.
+    - unfold eval_literal, a in Hfalse; simpl in Hfalse.
+      destruct excluded_middle_informative as [Hv_range|Hnot]; [|exfalso; exact (Hnot Hv)].
+      destruct excluded_middle_informative as [Hprec_v|Hnotprec_v].
+      + exfalso.
+        assert (Hneq : scc_of (v, true) <> scc_of (v, false))
+          by (apply scc_of_neq; auto; exact Hv_range).
+        assert (Hin1 : In (scc_of (v, true)) sccs)
+          by (eapply scc_of_spec; eauto; exact (conj Hv_range eq_refl)).
+        assert (Hin2 : In (scc_of (v, false)) sccs)
+          by (eapply scc_of_spec; eauto; exact (conj Hv_range eq_refl)).
+        discriminate.
+      + assert (Hneq : scc_of (v, true) <> scc_of (v, false))
+          by (apply scc_of_neq; auto; exact Hv_range).
+        assert (Hin1 : In (scc_of (v, true)) sccs)
+          by (eapply scc_of_spec; eauto; exact (conj Hv_range eq_refl)).
+        assert (Hin2 : In (scc_of (v, false)) sccs)
+          by (eapply scc_of_spec; eauto; exact (conj Hv_range eq_refl)).
+        destruct (Htotal (scc_of (v, true)) (scc_of (v, false)) Hin1 Hin2 Hneq)
+          as [Hord|Hord'];
+        [exact Hord
+        |exfalso; exact (Hnotprec_v Hord')].
+    - unfold eval_literal, a in Hfalse; simpl in Hfalse.
+      destruct excluded_middle_informative as [Hv_range|Hnot]; [|exfalso; exact (Hnot Hv)].
+      destruct excluded_middle_informative as [Hprec_v|Hnotprec_v]; [exact Hprec_v|discriminate]. }
+  assert (step_cond_or_eq : forall (l1 l2 : literal),
+    step g l1 l2 ->
+    (scc_of l1 = scc_of l2) \/
+    condensation_edge g sccs (scc_of l1) (scc_of l2)).
+  { intros l1 l2 Hstep.
+    destruct Hstep as [e Hstep].
+    destruct Hstep as [He Hx Hy Hfx Hsy].
+    subst l1 l2.
+    assert (Hvx : valid_literal numVars (dig_fst g e))
+      by (unfold g, implication_graph; simpl; exact Hx).
+    assert (Hvy : valid_literal numVars (dig_snd g e))
+      by (unfold g, implication_graph; simpl; exact Hy).
+    destruct (classic (scc_of (dig_fst g e) = scc_of (dig_snd g e))) as [Heq|Hneq];
+      [left; auto| right].
+    destruct (scc_of_spec (dig_fst g e) Hvx) as [Hin1 Hl1].
+    destruct (scc_of_spec (dig_snd g e) Hvy) as [Hin2 Hl2].
+    unfold condensation_edge.
+    repeat split; auto.
+    exists (dig_fst g e), (dig_snd g e); repeat split; auto.
+    unfold step; exists e.
+    exact (DigStepAux literal Z g e (dig_fst g e) (dig_snd g e) He Hx Hy eq_refl eq_refl). }
+  exists a.
+  unfold satisfies; intros [l1 l2] Hc.
+  destruct (classic (eval_literal a l1 = true \/ eval_literal a l2 = true)) as [Hdis|Hndis].
+  - destruct Hdis as [H|H]; auto.
+  - destruct (not_or_and _ _ Hndis) as [Hf1 Hf2].
+    apply Bool.not_true_is_false in Hf1.
+    apply Bool.not_true_is_false in Hf2.
+  assert (Hvalid_c : valid_clause numVars (l1, l2)) by (apply Hvalid; exact Hc).
+  destruct Hvalid_c as [Hv1 Hv2].
+  assert (Hv_neg1 : valid_literal numVars (negate l1)) by (apply valid_literal_negate; auto).
+  assert (Hv_neg2 : valid_literal numVars (negate l2)) by (apply valid_literal_negate; auto).
+  assert (Hprec_l1 : prec (scc_of l1) (scc_of (negate l1))) by (apply eval_false_prec; auto).
+  assert (Hprec_l2 : prec (scc_of l2) (scc_of (negate l2))) by (apply eval_false_prec; auto).
+  assert (Hstep_edges : step g (negate l1) l2 /\ step g (negate l2) l1)
+    by (apply (step_implication f numVars Hvalid (l1, l2) Hc)).
+  destruct Hstep_edges as [Hstep1 Hstep2].
+  assert (Hprec_dag1 : prec (scc_of (negate l1)) (scc_of l2) \/
+                       scc_of (negate l1) = scc_of l2).
+  { pose proof (step_cond_or_eq (negate l1) l2 Hstep1) as Hsc.
+    destruct Hsc as [Heq | Hce].
+    - right; exact Heq.
+    - left; apply Hcond_edge; exact Hce. }
+  assert (Hprec_dag2 : prec (scc_of (negate l2)) (scc_of l1) \/
+                       scc_of (negate l2) = scc_of l1).
+  { pose proof (step_cond_or_eq (negate l2) l1 Hstep2) as Hsc.
+    destruct Hsc as [Heq | Hce].
+    - right; exact Heq.
+    - left; apply Hcond_edge; exact Hce. }
+  assert (Hchain1 : prec (scc_of l1) (scc_of l2)).
+  { destruct Hprec_dag1 as [Hedge|Heq].
+    - apply (Htrans _ _ _ Hprec_l1 Hedge).
+    - rewrite <- Heq; exact Hprec_l1. }
+  assert (Hchain2 : prec (scc_of l2) (scc_of l1)).
+  { destruct Hprec_dag2 as [Hedge|Heq].
+    - apply (Htrans _ _ _ Hprec_l2 Hedge).
+    - rewrite <- Heq; exact Hprec_l2. }
+  assert (Hcycle : prec (scc_of l1) (scc_of l1))
+    by (apply (Htrans _ _ _ Hchain1 Hchain2)).
+  exfalso; exact (Hirrefl _ _ Hcycle Hcycle).
+Qed.
 
 End BACKWARD.
 
@@ -351,5 +559,6 @@ Proof.
   intros f numVars Hvalid.
   split.
   - apply forward; auto.
-  - admit.
-Admitted.
+  - intro Hnc.
+    exact (backward f numVars Hvalid Hnc).
+Qed.
